Added modified ALU

EbpfVerifierRangeAnalysis/Overflow.lean
@@ -1,21 +1,26 @@
 import Mathlib.Data.Int.Init
 
+def UInt32_max : UInt32 := UInt32.ofNat (2^32 - 1)
+def UInt_max : UInt64 := UInt64.ofNat (2^64 - 1)
+def Int32_max : Int32 := Int32.maxValue
+def Int_max : Int64 := Int64.maxValue
+
 @[simp]
 def unsignedCheckAddOverflow32 (a b : UInt32) : Bool :=
   let sum := a.toNat + b.toNat
-  sum ≥ UInt32.size
+  sum ≥ UInt32_max
 
 @[simp]
 def signedCheckAddOverflow32 (a b : Int32): Bool :=
   let sum := a.toNat + b.toNat
-  sum ≥ Int32.size
+  sum ≥ Int32_max
 
 @[simp]
 def unsignedCheckAddOverflow(a b : UInt64) : Bool :=
   let sum := a.toNat + b.toNat
-  sum ≥ UInt64.size
+  sum ≥ UInt_max
 
 @[simp]
 def signedCheckAddOverflow (a b : Int64) : Bool :=
   let sum := a.toNat + b.toNat
-  sum ≥ UInt64.size
+  sum ≥ Int_max
